common/SetoidListFacts.v
@@ -1,25 +1,60 @@
 (** * More Facts about Setoid Lists *)
 
 Require Import common.Coqlib.
+Require Import common.ListPlus.
 Require Import common.FstSplit.
 
-Lemma setoidl_eq_in :
-  forall {A B : Type} l {eqk : A -> A -> Prop} {eqv : B -> B -> Prop} a a' b ,
-    Equivalence eqk -> 
-    eqk a a' ->
+(** ** Fst and Split Facts for Setoid Lists *)
+
+(** If a couple (a, b) is in the list of couples l 
+    then a is in (fst (split l)). *)
+
+Lemma InA_fst_split {A B : Type} :
+  forall {eqk : A -> A -> Prop} {eqv : B -> B -> Prop} {a l} (b : B),
     let eqkv := (fun x y => eqk (fst x) (fst y) /\ eqv (snd x) (snd y)) in
-    InA eqkv (a, b) l ->
-    InA eqkv (a', b) l.
+    InA eqkv (a, b) l -> InA eqk a (fst (split l)).
 Proof.
   induction l.
-
-  - inversion 3.
-  - intros; destruct a.
-    apply InA_cons.
-    inversion_clear H1.
-    + left; firstorder.
-    + right; apply IHl with (a := a0); auto.
+  - intros; inversion H.
+  - elim a0; intros; rewrite fst_split_cons_app; simpl.
+    inversion_clear H; apply InA_cons.
+    + firstorder.
+    + right; apply IHl with (b := b0); auto.
 Qed.
+
+Hint Resolve InA_fst_split : setoidl.
+
+(* Version of [not_in_fst_split] for setoid lists. *)
+
+Lemma not_InA_fst_split {A B : Type} :
+  forall {l : list (A * B)} {eqk : A -> A -> Prop} {eqv : B -> B -> Prop} {a : A},
+    ~InA eqk a (fst (split l)) ->
+    let eqkv := (fun x y => eqk (fst x) (fst y) /\ eqv (snd x) (snd y)) in
+    (forall b : B, ~InA eqkv (a, b) l).
+Proof.
+  induction l.
+  - intros; intros Hin; inversion Hin.
+  - elim a; intros; intros Hin.
+    specialize (InA_fst_split b0 Hin) as Hnotin_a1.
+    contradiction.
+Qed.
+
+Hint Resolve not_InA_fst_split : setoidl.
+
+Lemma InA_eqk :
+  forall {A B : Type} {eqk : A -> A -> Prop} (eqv : B -> B -> Prop) {x y z l},
+    eqk x y ->
+    Equivalence eqk ->
+    let eqkv := fun x y => eqk (fst x) (fst y) /\ eqv (snd x) (snd y) in
+    InA eqkv (x, z) l ->
+    InA eqkv (y, z) l.
+Proof.
+  induction 3;
+    [ destruct y0 as (a, b); apply InA_cons_hd; firstorder
+    | apply InA_cons_tl; auto].
+Qed.
+
+Hint Resolve InA_eqk : setoidl.
 
 Lemma NoDupA_fs_eqk_eq (A : Type) {B : Type} :
   forall {eqk : A -> A -> Prop} {l : list (A * B)} {a b b'},
@@ -60,19 +95,35 @@ Proof.
                       | [ H: ~InA _ _ _ |- _ ] =>
                         apply H
                       end.
-      apply (@setoidl_in_fst_split A B eqk eq a1 l b').
-      eapply setoidl_eq_in with (a := a0); eauto.
-      firstorder.
+      apply (@InA_fst_split A B eqk eq a1 l b').
+      eapply InA_eqk; eauto; firstorder.
 
     + elimtype False; lazymatch goal with
                       | [ H: ~InA _ _ _ |- _ ] =>
                         apply H
                       end.
-      apply (@setoidl_in_fst_split A B eqk eq a1 l b).
-      eapply setoidl_eq_in with (a := a0); eauto.
-      firstorder.
+      apply (@InA_fst_split A B eqk eq a1 l b).
+      eapply InA_eqk; eauto; firstorder.
 
     + eapply IHl; eauto.
 Qed.
 
-Hint Rewrite NoDupA_fs_eqk_eq : core.
+Hint Rewrite NoDupA_fs_eqk_eq : setoidl.
+
+Lemma InA_setv :
+  forall {A B : Type} {x y : A} {z v : B} {eqk eqv l} {eqk_dec : forall x y, {eqk x y} + {~eqk x y}},
+    let eqkv := (fun x y => eqk (fst x) (fst y) /\ eqv (snd x) (snd y)) in
+    InA eqkv (x, z) l ->
+    ~eqk x y ->
+    Equivalence eqk ->
+    InA eqkv (x, z) (setv eqk_dec y v l).
+Proof.
+  induction 1.
+  
+  all: destruct y0; intros; simpl; destruct (eqk_dec y a); auto.
+  destruct H as (Heqk, Heqv); simpl in Heqk.
+  apply (Equivalence_Symmetric y a) in e.
+  apply (Equivalence_Transitive x a y) in e; [contradiction | auto].
+Qed.
+
+Hint Resolve InA_setv : setoidl.
