common/StateAndErrorMonadTactics.v
@@ -1,0 +1,115 @@
+(** * Tactics for the State-and-Error Monad *)
+
+Require Import common.StateAndErrorMonad.
+
+Remark Bind_inversion:
+  forall (state A B : Type) (f: Mon A) (g: A -> Mon B)
+         (y: B) (s1 s3: state),
+    Bind f g s1 = OK y s3 ->
+    exists x, exists s2,
+        f s1 = OK x s2 /\ g x s2 = OK y s3.
+Proof.
+  intros *. unfold Bind. destruct (f s1); intros.
+  discriminate.
+  exists a; exists s.
+  destruct (g a s); inversion H; auto.
+Qed.
+
+Ltac monadInv1 H :=
+  match type of H with
+  | (OK _ _ = OK _ _) =>
+    inversion H; clear H; try subst
+  | (Get _ = OK _ _) =>
+    inversion H; clear H; try subst
+  | (Put _ _ = OK _ _) =>
+    inversion H; clear H; try subst
+  | (Ret _ _ = OK _ _) =>
+    inversion H; clear H; try subst
+  | (Error _ = OK _ _) =>
+    discriminate
+  | (Bind ?F ?G ?S = OK ?X ?S') =>
+    let x := fresh "x" in
+    let s := fresh "s" in
+    let EQ1 := fresh "EQ" in
+    let EQ2 := fresh "EQ" in
+    destruct (Bind_inversion _ _ _ F G X S S' H) as [x [s [EQ1 EQ2]]];
+    clear H;
+    try (monadInv1 EQ2)
+  end.
+
+Ltac monadInv H :=
+  match type of H with
+  | (Get _ = OK _ _) => monadInv1 H
+  | (Put _ = OK _ _) => monadInv1 H
+  | (Ret _ _ = OK _ _) => monadInv1 H
+  | (Error _ = OK _ _) => monadInv1 H
+  | (Bind ?F ?G ?S = OK ?X ?S') => monadInv1 H
+  | (?F _ _ _ _ _ _ _ _ = OK _ _) =>
+    ((progress simpl in H) || unfold F in H); monadInv1 H
+  | (?F _ _ _ _ _ _ _ = OK _ _) =>
+    ((progress simpl in H) || unfold F in H); monadInv1 H
+  | (?F _ _ _ _ _ _ = OK _ _) =>
+    ((progress simpl in H) || unfold F in H); monadInv1 H
+  | (?F _ _ _ _ _ = OK _ _) =>
+    ((progress simpl in H) || unfold F in H); monadInv1 H
+  | (?F _ _ _ _ = OK _ _) =>
+    ((progress simpl in H) || unfold F in H); monadInv1 H
+  | (?F _ _ _ = OK _ _) =>
+    ((progress simpl in H) || unfold F in H); monadInv1 H
+  | (?F _ _ = OK _ _) =>
+    ((progress simpl in H) || unfold F in H); monadInv1 H
+  | (?F _ = OK _ _) =>
+    ((progress simpl in H) || unfold F in H); monadInv1 H
+  end.
+
+Ltac monadFullInv1 H :=
+  match type of H with
+  | (OK _ _ = OK _ _)    => monadInv1 H
+  | (Get _ = OK _ _)     => monadInv1 H
+  | (Put _ _ = OK _ _)   => monadInv1 H
+  | (Error _ = OK _ _) => monadInv1 H
+  | (Ret _ _ = OK _ _) => monadInv1 H
+  | (Bind ?F ?G ?S = OK ?X ?S') =>
+    let x := fresh "x" in
+    let s := fresh "s" in
+    let EQ1 := fresh "EQ" in
+    let EQ2 := fresh "EQ" in
+    destruct (Bind_inversion _ _ _ F G X S S' H) as [x [s [EQ1 EQ2]]];
+    clear H;
+    try (monadFullInv1 EQ2);
+    try (monadFullInv1 EQ1)
+  end.
+
+Ltac monadFullInv H :=
+  match type of H with
+  | (Get _ = OK _ _) => monadFullInv1 H
+  | (Put _ _ = OK _ _) => monadFullInv1 H
+  | (Ret _ _ = OK _ _) => monadFullInv1 H
+  | (Error _ = OK _ _) => monadFullInv1 H
+  | (Bind ?F ?G ?S = OK ?X ?S') =>
+    let x := fresh "x" in
+    let s := fresh "s" in
+    let EQ1 := fresh "EQ" in
+    let EQ2 := fresh "EQ" in
+    destruct (Bind_inversion _ _ _ F G X S S' H) as [x [s [EQ1 EQ2]]];
+    clear H;
+    try (monadFullInv EQ2);
+    try (monadFullInv EQ1)
+  (* | (Bind ?F ?G ?S = OK ?X ?S') => monadFullInv1 H *)
+  | (?F _ _ _ _ _ _ _ _ = OK _ _) =>
+    ((progress simpl in H) || unfold F in H); monadFullInv H
+  | (?F _ _ _ _ _ _ _ = OK _ _) =>
+    ((progress simpl in H) || unfold F in H); monadFullInv H
+  | (?F _ _ _ _ _ _ = OK _ _) =>
+    ((progress simpl in H) || unfold F in H); monadFullInv H
+  | (?F _ _ _ _ _ = OK _ _) =>
+    ((progress simpl in H) || unfold F in H); monadFullInv H
+  | (?F _ _ _ _ = OK _ _) =>
+    ((progress simpl in H) || unfold F in H); monadFullInv H
+  | (?F _ _ _ = OK _ _) =>
+    ((progress simpl in H) || unfold F in H); monadFullInv H
+  | (?F _ _ = OK _ _) =>
+    ((progress simpl in H) || unfold F in H); monadFullInv H
+  | (?F _ = OK _ _) =>
+    ((progress simpl in H) || unfold F in H); monadFullInv H
+  end.
