sitpn/dp/SitpnWellDefinedTactics.v
@@ -1,0 +1,21 @@
+(** * Tactics for the IsWellDefined Predicate *)
+
+Require Import sitpn.dp.SitpnWellDefined.
+
+Ltac build_nodup_places H :=
+  lazymatch type of H with
+  | IsWellDefined ?sitpn =>
+    let Hndpls := fresh "NoDupPlaces" in
+    destruct (H) as (_, (_, (_, (_, (_, (_, (Hndpls, _))))))); Hndpls
+  | _ => let to := type of H in
+         fail "Term" H "is of type" to "while it is expected to be of type IsWelldefined ?sitpn"
+  end.
+
+Ltac get_nodup_places H :=
+  lazymatch type of H with
+  | IsWellDefined ?sitpn =>
+    constr:(proj1 (proj2 (proj2 (proj2 (proj2 (proj2 (proj2 H)))))))
+  | _ => let to := type of H in
+         fail "Term" H "is of type" to "while it is expected to be of type IsWelldefined ?sitpn"
+  end.
+
