sitpn/simpl/SitpnRisingEdgeMarkingComplete.v
@@ -6,11 +6,6 @@ Require Import simpl.SitpnSemantics.
 Require Import simpl.SitpnTactics.
 Require Import simpl.SitpnCoreLemmas.
 
-(* Import misc. lemmas, tactics and definitions. *)
-
-
-
-
 (* Import lemmas about marking. *)
 
 Require Import simpl.SitpnWellDefMarking.
@@ -244,7 +239,7 @@ Section MapUpdateMarkingPreComplete.
           assert (Hneq_ap : a <> p).
           {
             apply NoDup_cons_iff, proj1 in Hnodup_prepl.
-            apply (not_in_in_diff a p pre_places (conj Hnodup_prepl Hin_p_prepl)).
+            apply (not_in_in_diff (conj Hnodup_prepl Hin_p_prepl)).
           }
           
           rewrite (modify_m_in_if_diff marking a Nat.sub (pre sitpn t a) m'
@@ -544,7 +539,7 @@ Section MapUpdateMarkingPostComplete.
           assert (Hneq_ap : a <> p).
           {
             apply NoDup_cons_iff, proj1 in Hnodup_postpl.
-            apply (not_in_in_diff a p post_places (conj Hnodup_postpl Hin_p_postpl)).
+            apply (not_in_in_diff (conj Hnodup_postpl Hin_p_postpl)).
           }
           
           rewrite (modify_m_in_if_diff marking a Nat.add (post sitpn t a) m'
@@ -730,7 +725,7 @@ Section MapUpdateMarkingComplete.
         -- intro Heq_diff; elim Heq_diff; reflexivity.
       + simpl; case (Nat.eq_dec a t).
         -- rewrite NoDup_cons_iff in Hnodup_l; apply proj1 in Hnodup_l.
-           specialize (not_in_in_diff t a tail (conj Hnodup_l Hin_a_tl)) as Hdiff_ta.
+           specialize (not_in_in_diff (conj Hnodup_l Hin_a_tl)) as Hdiff_ta.
            intro Heq_at; symmetry in Heq_at; contradiction.
         -- intro Hdiff_at.
            simpl; symmetry; rewrite Nat.add_comm.
@@ -774,7 +769,7 @@ Section MapUpdateMarkingComplete.
         - intro Hin_tl; specialize (in_cons t t0 tail Hin_tl) as Hin_t0_ctl.
           rewrite NoDup_cons_iff in Hnodup_l.
           apply proj1 in Hnodup_l.
-          specialize (not_in_in_diff t t0 tail (conj Hnodup_l Hin_tl)) as Hdiff_tt0.
+          specialize (not_in_in_diff (conj Hnodup_l Hin_tl)) as Hdiff_tt0.
           apply not_eq_sym in Hdiff_tt0.
           rewrite Hequiv in Hin_t0_ctl.
           rewrite in_remove_iff; apply (conj Hin_t0_ctl Hdiff_tt0).
